cleanup of Eisbach_Methods. Adding some documentation and some more methods

lib/Eisbach_Methods.thy
@@ -1,4 +1,16 @@
-(* Some useful boilerplate methods for Eisbach *)
+(*
+ * Copyright 2014, NICTA
+ *
+ * This software may be distributed and modified according to the terms of
+ * the BSD 2-Clause license. Note that NO WARRANTY is provided.
+ * See "LICENSE_BSD2.txt" for details.
+ *
+ * @TAG(NICTA_BSD)
+ *)
+
+(*
+   Methods and method combinators that are built using Eisbach.
+*)
 
 theory Eisbach_Methods
 imports "~~/src/HOL/Eisbach/Eisbach_Tools" 
@@ -7,6 +19,24 @@ imports "~~/src/HOL/Eisbach/Eisbach_Tools"
 begin
 
 
+section \<open>Debugging methods\<close>
+
+method print_concl = (match conclusion in P for P \<Rightarrow> \<open>print_term P\<close>)
+
+method_setup print_raw_goal = \<open>Scan.succeed (fn ctxt => fn facts => 
+  (fn st => (Output.writeln (Display.string_of_thm ctxt st); Seq.single ([],st))))\<close>
+
+
+method_setup print_headgoal = 
+  \<open>Scan.succeed (fn ctxt =>
+   SIMPLE_METHOD
+    (SUBGOAL (fn (t,_) => 
+     (Output.writeln 
+     (Pretty.string_of (Syntax.pretty_term ctxt t)); all_tac)) 1))\<close>
+
+section \<open>Simple Combinators\<close>
+
+method_setup defer_tac = \<open>Scan.succeed (fn _ => SIMPLE_METHOD (defer_tac 1))\<close>
 
 method_setup all =
  \<open>Method_Closure.parse_method >> (fn m => fn ctxt => fn facts =>
@@ -16,18 +46,12 @@ method_setup all =
        |> Method_Closure.method_evaluate m ctxt facts
        |> Seq.map (Goal.unrestrict i o snd)
 
-   in EMPTY_CASES (ALLGOALS tac) end)
+   in SIMPLE_METHOD (ALLGOALS tac) facts end)
 \<close>
 
-method print_concl = (match conclusion in P for P \<Rightarrow> \<open>print_term P\<close>)
-
-method_setup print_goal = \<open>Scan.succeed (fn ctxt => fn facts => 
-  (fn st => (Output.writeln (Display.string_of_thm ctxt st); Seq.single ([],st))))\<close>
-
-
-
-
-(* lift methods into logical tests *)
+text \<open>The following @{text fails} and @{text succeeds} methods protect the goal from the effect
+      of a method, instead simply determining whether or not it can be applied to the current goal.
+      The @{text fails} method inverts success, only succeeding if the given method would fail.\<close>
 
 method_setup fails =
  \<open>Method_Closure.parse_method >> (fn m => fn ctxt => fn facts =>
@@ -37,7 +61,7 @@ method_setup fails =
           SOME _ => Seq.empty
         | NONE => Seq.single st')
 
-   in EMPTY_CASES fail_tac end)
+   in SIMPLE_METHOD fail_tac facts end)
 \<close>
 
 method_setup succeeds =
@@ -48,14 +72,25 @@ method_setup succeeds =
           SOME (st'',_) => Seq.single st'
         | NONE => Seq.empty)
 
-   in EMPTY_CASES can_tac end)
+   in SIMPLE_METHOD can_tac facts end)
 \<close>
 
-(* focus without matching *)
+text \<open>This method wraps up the "focus" mechanic of match without actually doing any matching.
+      We need to consider whether or not there are any assumptions in the goal,
+      as premise matching fails if there are none.
+
+      If the @{text fails} method is removed here, then backtracking will produce
+      a set of invalid results, where only the conclusion is focused despite
+      the presence of subgoal premises.
+      \<close>
 
 method focus_concl methods m =
   ((fails \<open>erule thin_rl\<close>, match conclusion in _ \<Rightarrow> \<open>m\<close>)
-  | match premises in H:_ (multi) \<Rightarrow> \<open>m\<close>)
+  | match premises (local) in H:_ (multi) \<Rightarrow> \<open>m\<close>)
+
+section \<open>Advanced combinators\<close>
+
+subsection \<open>Protecting goal elements (assumptions or conclusion) from methods\<close>
 
 context
 begin
@@ -79,13 +114,74 @@ method only_concl methods m = (focus_concl \<open>m\<close>)
 
 end
 
+notepad begin
+ fix D C
+  assume DC:"D \<Longrightarrow> C"
+  have "D \<and> D \<Longrightarrow> C \<and> C"
+  apply (only_asm \<open>simp\<close>) -- "stash conclusion before applying method"
+  apply (only_concl \<open>simp add: DC\<close>) -- "hide premises from method"
+  by (rule DC)
+
+end
+
+subsection \<open>Safe subgoal folding (avoids expanding meta-conjuncts)\<close>
+
+text \<open>Isabelle's goal mechanism wants to aggressively expand meta-conjunctions if they
+      are the top-level connective. This means that @{text fold_subgoals} will immediately
+      be unfolded if there are no common assumptions to lift over.
+
+      This method simply ensures that this is the case by inserting a dummy assumption
+      as the first assumption to all subgoals, so that after folding the goal
+      looks like this: @{term "dummy_asm ==> A &&& B"}. The inner method is then
+      executed on the resulting goal, without expanding the conjuncts.
+
+      The inner method should probably clear this dummy assumption internally at
+      some point (using the provided @{text clear_dummy_asm}, 
+      but only when it doesn't need the conjunction to persist.\<close>
+
 context begin
 
-private definition "goal_tag (x :: unit) \<equiv> TERM x"
+private definition "dummy_asm == True"
+private lemma dummy_asm: "dummy_asm" by (simp add: dummy_asm_def)
+
+method clear_dummy_asm = (erule thin_rl[of dummy_asm])?
+
+method safe_fold_subgoals methods m =
+  (all \<open>insert dummy_asm, rotate_tac -1\<close>,
+   fold_subgoals,
+   (m ; clear_dummy_asm))
+
+end
+
+notepad begin
+  fix D C E
+  
+  assume DC: "D &&& C"
+  have "D" "C"
+  apply -
+  by (safe_fold_subgoals \<open>rule DC\<close>)
+
+end
+
+
+section \<open>Utility methods\<close>
+  
+
+subsection \<open>Finding a goal based on successful application of a method\<close>
+
+text \<open>This method works by creating "tagged" subgoals in order to use the + operator
+      to iterate over all goals without looping indefinitely.
+      Effectively this looks like a while-loop, which breaks out when either
+      the "end" subgoal is found or when the method succeeds and the "success"
+      subgoal is found.\<close>
+
+context begin
+
+private definition "goal_tag (x :: unit) \<equiv> Trueprop True"
 
 private lemma goal_tagI: "PROP goal_tag x"
   unfolding goal_tag_def
-  by (rule termI)
+  by simp
 
 private method make_tag_goal for tag_id :: unit = (rule thin_rl[of "PROP goal_tag tag_id"])
 
@@ -95,8 +191,6 @@ private definition "goals_end \<equiv> ()"
 private definition "method_succeed \<equiv> ()"
 private definition "method_failure \<equiv> ()"
 
-
-private method defer_tac = tactic \<open>defer_tac 1\<close>
 
 method find_goal methods m = 
   (make_tag_goal goals_end, 
@@ -109,8 +203,6 @@ method find_goal methods m =
 
 end
 
-(* examples *)
-
 notepad begin
 
   fix A B
@@ -122,24 +214,91 @@ notepad begin
     by (rule A)+
 
   have "A \<and> A" "A \<and> A" "B"
-    apply (find_goal \<open>fails \<open>simp\<close>\<close>) (* find the first goal which cannot be simplified *)
+    apply (find_goal \<open>fails \<open>simp\<close>\<close>) -- "find the first goal which cannot be simplified"
     apply (rule B)
     by (simp add: A)+
 
   have  "B" "A" "A \<and> A"
-    apply (find_goal \<open>succeeds \<open>simp\<close>\<close>) (* find the first goal which can be simplified (without doing so) *)
+    apply (find_goal \<open>succeeds \<open>simp\<close>\<close>) -- "find the first goal which can be simplified (without doing so)"
     apply (rule conjI)
     by (rule A B)+
-
-
-  fix D C
-  assume DC:"D \<Longrightarrow> C"
-  have "D \<and> D \<Longrightarrow> C \<and> C"
-  apply (only_asm \<open>simp\<close>) (* stash conclusion before applying method *)
-  apply (only_concl \<open>simp add: DC\<close>) (* hide premises from method *)
-  by (rule DC)
+ 
 end
-    
+
+
+subsection \<open>Remove redundant subgoals\<close>
+
+text \<open>Tries to solve subgoals by assuming the others and then using the given method.
+      Backtracks over all possible re-orderings of the subgoals.\<close>
+
+context begin
+
+definition "protect (PROP P) \<equiv> P"
+
+lemma protectE: "PROP protect P \<Longrightarrow> (PROP P \<Longrightarrow> PROP R) \<Longrightarrow> PROP R" by (simp add: protect_def)
+
+private lemmas protect_thin = thin_rl[where V="PROP protect P" for P]
+
+private lemma context_conjI_protected:
+  assumes P: "PROP P"
+  assumes PQ: "PROP protect (PROP P) \<Longrightarrow> PROP Q"
+  shows
+  "PROP P &&& PROP Q"
+   apply -
+   apply (rule P)
+  apply (rule PQ)
+  apply (simp add: protect_def)
+  by (rule P)
+
+private lemma conjunction_sym: "PROP P &&& PROP Q \<Longrightarrow> PROP Q &&& PROP P"
+  apply (frule conjunctionD1)
+  apply (drule conjunctionD2)
+  apply (rule conjunctionI)
+  by assumption+
+
+private lemma conjunctionE:
+  assumes PQ: "PROP P &&& PROP Q"
+  assumes PQR: "PROP P \<Longrightarrow> PROP Q \<Longrightarrow> PROP R"
+  shows
+  "PROP R"
+  apply (rule PQR)
+  apply (rule PQ[THEN conjunctionD1])
+  by (rule PQ[THEN conjunctionD2])
+  
+private lemmas context_conjI_protected' = context_conjI_protected[THEN conjunction_sym]
+
+method distinct_subgoals_strong methods m = 
+  (safe_fold_subgoals \<open>
+   (intro context_conjI_protected context_conjI_protected'; 
+     (((elim protectE conjunctionE)?,clear_dummy_asm, solves \<open>m\<close>)
+     | (elim protect_thin)?))\<close>)?
+
+end
+
+
+notepad begin
+  {
+  fix A B C
+  assume A: "A"
+  have "A" "B \<Longrightarrow> A"
+  apply (distinct_subgoals_strong \<open>assumption\<close>)
+  by (rule A)
+
+  have "B \<Longrightarrow> A" "A" 
+  by (distinct_subgoals_strong \<open>assumption\<close>, rule A) -- "backtracking required here"
+  }
+
+  {
+  fix A B C
+  
+  assume B: "B"
+  assume BC: "B \<Longrightarrow> C" "B \<Longrightarrow> A"
+  have "A" "B \<longrightarrow> (A \<and> C)" "B"
+  apply (distinct_subgoals_strong \<open>simp\<close>, rule B) -- "backtracking required here"
+  by (simp add: BC)
+  
+  }
+end
 
 
 end
